documented knowledge soundness batch

src/KZG_BatchOpening_binding.thy
@@ -1,24 +1,38 @@
 theory KZG_BatchOpening_binding
 
-imports KZG_eval_bind KZG_BatchOpening_correct tBSDH_assumption
+imports KZG_eval_bind KZG_BatchOpening_correct tBSDH_assumption SPMF_ext
 begin
 
 locale bind_game_def = KZG_BatchOpening_correct
 begin
 
+section \<open>Definitions for the evaluation binding game for the batched KZG\<close>
+
+text \<open>We define the evaluation binding game, the reduction to the t-BSDH assumption as well as any 
+functions needed to construct them in this locale. This file contains another locale below which 
+contains the proof.\<close>
+
+text \<open>valid_msg ensures that the supplied witness w_i is a group element of Gp. 
+Sadly cyclic groups are not constructed by type, which is why this check is necessary. 
+A element of type 'a is not necessarily a group element of Gp.\<close>
 definition valid_msg :: "'e eval_value \<Rightarrow> 'a eval_witness \<Rightarrow> bool" where 
   "valid_msg \<phi>_i w_i = (w_i \<in> carrier G\<^sub>p)"
 
+text \<open>valid_batch_msg similarly to valid_msg ensures that the supplied witness w_B is a group 
+element of Gp. Furthermore, it ensures that the degree of r(x) is less than |B|, which is a 
+prerequisist for r(x) to be valid as r(x) is the remainder of a divison by \<Prod>i\<in>B.(x-i). 
+Additionally, it checks that B is not revealing more points than max_deg.\<close>
 definition valid_batch_msg :: "'e polynomial \<Rightarrow> 'a eval_witness \<Rightarrow> 'e eval_position set \<Rightarrow> bool" where 
   "valid_batch_msg r_x w_B B = (w_B \<in> carrier G\<^sub>p \<and> degree r_x < card B \<and> card B < max_deg)"
                     
-subsection \<open>Game definition\<close>
+subsection \<open>Game definition\<close> 
 
 type_synonym ('a', 'e')  adversary = 
   "'a' pk \<Rightarrow> 
  ('a' commit \<times> 'e' eval_position \<times> 'e' eval_value \<times> 'a' eval_witness \<times> 'e' eval_position set 
   \<times> 'a' eval_witness \<times> 'e' polynomial) spmf"
 
+text \<open>This is the formalized evaluation binding game\<close>
 definition bind_game :: "('a, 'e) adversary \<Rightarrow> bool spmf"
   where "bind_game \<A> = TRY do {
   PK \<leftarrow> KeyGen;
@@ -28,21 +42,50 @@ definition bind_game :: "('a, 'e) adversary \<Rightarrow> bool spmf"
   let b' = VerifyEvalBatch PK C B r_x w_B;
   return_spmf (b \<and> b')} ELSE return_spmf False"
 
+text \<open>The advantage of the adversary over the evaluation binding game is the probabillity that it 
+wins.\<close>
 definition bind_advantage :: "('a, 'e) adversary \<Rightarrow> real"
   where "bind_advantage \<A> \<equiv> spmf (bind_game \<A>) True"
                                                         
-subsection \<open>t-SDH game\<close>
+subsection \<open>t-BSDH game\<close>
 
+text \<open>We instantiate the t-BSDH game for the pairing e, with  the group Gp as preimage group and GT 
+as target group.\<close>
 sublocale t_BSDH: t_BSDH G\<^sub>p G\<^sub>T max_deg "of_int_mod_ring \<circ> int" "pow_mod_ring G\<^sub>p" "pow_mod_ring G\<^sub>T" e
   unfolding t_BSDH_def 
   using G\<^sub>T.cyclic_group_axioms G\<^sub>p.cyclic_group_axioms by presburger
 
-subsection \<open>Defining a reduction game to t-SDH\<close>
+subsection \<open>Defining a reduction game to t-BSDH\<close>
 
-fun bind_reduction
+text \<open>The reduction function takes a adversary for the evaluation binding game and returns an 
+adversary for the t-BSDH game. Specifically, the reduction uses the evaluation binding adversary to 
+construct a winning strategy for the t-BSDH game (i.e. to win it every time).
+Essentially, it uses the fact that the values supplied by the adversary already break the t-BSDH 
+assumption.\<close>
+fun reduction
   :: "('a, 'e) adversary \<Rightarrow> ('a,'e,'c) t_BSDH.adversary"                     
 where
-  "bind_reduction \<A> PK = do {
+  "reduction \<A> PK = do {
+   (C, i, \<phi>_i, w_i, B, w_B, r_x) \<leftarrow> \<A> PK;
+  let p' = g_pow_PK_Prod PK (prod (\<lambda>i. [:-i,1:]) B div [:-i,1:]);
+  let r' = g_pow_PK_Prod PK ((r_x - [:poly r_x i:]) div [:-i,1:]);
+  return_spmf (-i::'e mod_ring, (e p' w_B \<otimes>\<^bsub>G\<^sub>T\<^esub> e (r' \<div>\<^bsub>G\<^sub>p\<^esub> w_i) \<^bold>g) ^\<^bsub>G\<^sub>T\<^esub> (1/(\<phi>_i - poly r_x i))) }"
+
+end
+
+text \<open>This locale captures the proof for the definitions provided earlier.
+Note, the proof is structured analogly to the normal KZG's evaluation bidning proof.\<close>
+locale bind_game_proof = bind_game_def
+begin
+
+text \<open>The reduction adversary extended for asserts that 
+are present in the evalutaion binding game. We use this definition to show equivalence to 
+the evaluation binding  game. Later on we can then easily over-estimate the probability 
+from this extended version to the normal reduction.\<close>
+fun ext_reduction
+  :: "('a, 'e) adversary \<Rightarrow> ('a,'e,'c) t_BSDH.adversary"                     
+where
+  "ext_reduction \<A> PK = do {
    (C, i, \<phi>_i, w_i, B, w_B, r_x) \<leftarrow> \<A> PK;
   _ :: unit \<leftarrow> assert_spmf (i \<in> B \<and> \<phi>_i \<noteq> poly r_x i \<and> valid_msg \<phi>_i w_i \<and> valid_batch_msg r_x w_B B
                             \<and> VerifyEval PK C i \<phi>_i w_i \<and> VerifyEvalBatch PK C B r_x w_B);
@@ -50,7 +93,9 @@ where
   let r' = g_pow_PK_Prod PK ((r_x - [:poly r_x i:]) div [:-i,1:]);
   return_spmf (-i::'e mod_ring, (e p' w_B \<otimes>\<^bsub>G\<^sub>T\<^esub> e (r' \<div>\<^bsub>G\<^sub>p\<^esub> w_i) \<^bold>g) ^\<^bsub>G\<^sub>T\<^esub> (1/(\<phi>_i - poly r_x i))) }"
 
-text \<open>An alternative but equivalent game for the binding game. 
+subsubsection \<open>helping lemmas\<close>
+
+text \<open>An alternative but equivalent game for the evaluation binding game. 
 This alternative game capsulates the 
 event that the Adversary wins in the assert_spmf statement.
 It's a closely adapted proof from Sigma_Commit_Crypto.Commitment_Schemes bind_game_alt_def\<close>
@@ -103,22 +148,9 @@ proof -
   finally show ?thesis .
 qed
 
-end
-
-locale bind_game_proof = bind_game_def
-begin
-
-lemma assert_anding: "TRY do {
-          _ :: unit \<leftarrow> assert_spmf (a);
-            _ :: unit \<leftarrow> assert_spmf (b);
-            return_spmf True
-        } ELSE return_spmf False 
-    = TRY do {
-          _ :: unit \<leftarrow> assert_spmf (a \<and> b);
-          return_spmf True
-      } ELSE return_spmf False"
-  by (simp add: try_bind_assert_spmf) 
-
+text \<open>show that VerifyEvalBatch of B and r(x) and VerifEval on i\<in>B and \<phi>_i suhc that \<phi>_i \<noteq> r(x) 
+implies that the t-BSDH is broken.
+This lemma captures that the adversaries messages already break the t-BSDH assumption.\<close>
 lemma verifys_impl_t_BSDH_break: 
   assumes 
     "i \<in> B \<and>  \<phi>_i \<noteq> poly r_x i \<and> valid_msg \<phi>_i w_i \<and> valid_batch_msg r_x w_B B \<and>
@@ -151,7 +183,9 @@ proof -
   then have p'_x_p_x: "(\<Prod>i\<in>B. [:- i, 1:]) = p'_x *  [:- i, 1:]"
     using assms 
     by (metis (no_types, lifting) Groups.mult_ac(2) arith_extra_simps(6) i_in_B_prod_B_zero nonzero_mult_div_cancel_left one_neq_zero pCons_eq_0_iff synthetic_div_correct')
-  
+
+  text \<open>the proof is essentially rearranging equations, an outline can be found in the batched versions
+  evaluation binding proof section in the thesis paper.\<close>
   from assms have "e w_i (map (\<lambda>t. \<^bold>g ^ \<alpha> ^ t) [0..<max_deg + 1] ! 1 \<otimes> inv (\<^bold>g ^ i)) \<otimes>\<^bsub>G\<^sub>T\<^esub> e \<^bold>g \<^bold>g ^\<^bsub>G\<^sub>T\<^esub> \<phi>_i
     = e (g_pow_PK_Prod (map (\<lambda>t. \<^bold>g ^ \<alpha> ^ t) [0..<max_deg + 1]) (\<Prod>i\<in>B. [:- i, 1:])) w_B \<otimes>\<^bsub>G\<^sub>T\<^esub>
   e \<^bold>g (g_pow_PK_Prod (map (\<lambda>t. \<^bold>g ^ \<alpha> ^ t) [0..<max_deg + 1]) r_x)" (is "?lhs = ?rhs")
@@ -173,7 +207,7 @@ proof -
     by argo
   then have "y*(\<alpha>-i) + \<phi>_i = (poly (\<Prod>i\<in>B. [:- i, 1:]) \<alpha>)*b + poly r_x \<alpha>"
     using e_bilinear e_linear_in_snd by force
-  text \<open>mimicking steps from batching opening binding proof in the paper. See Appendix C.3\<close>
+  text \<open>mimicking steps from batching opening binding proof in the orginal paper. See Appendix C.3 in [KZG10]\<close>
   then have "(poly (\<Prod>i\<in>B. [:- i, 1:]) \<alpha>)*b - (\<alpha>-i)*y = \<phi>_i -  poly r_x \<alpha>"
     by (metis (no_types, lifting) add_diff_cancel_left' add_diff_cancel_right' add_diff_eq mult.commute)
   then have "(poly (\<Prod>i\<in>B. [:- i, 1:]) \<alpha>)*b - (\<alpha>-i)*y = \<phi>_i - (poly r'_x \<alpha>)*(\<alpha>-i) - poly [:poly r_x i:] \<alpha>"
@@ -221,6 +255,11 @@ proof -
   show ?thesis by fastforce
 qed
 
+subsection \<open>literal helping lemma\<close>
+
+text \<open>CryptHOL has some difficulties with simplifying, thus we need to use literal helping lemmas, 
+that state the equalities we want to exchange literally.\<close>
+
 lemma literal_helping: 
   "(i \<in> (B::'e eval_position set) \<and>
                     (\<phi>_i:: 'e eval_value) \<noteq> (poly r_x i:: 'e eval_value) \<and>
@@ -245,9 +284,11 @@ lemma literal_helping:
                      w_B)"
   using verifys_impl_t_BSDH_break by fast
 
+subsection \<open>KZG eval bind game to reduction game - equivalence theorem\<close>
 
-theorem bind_game_eq_t_BSDH_red:
-  shows "bind_game \<A> = t_BSDH.game (bind_reduction \<A>)"
+text \<open>We show that the binding game is equivalent to the t-BSDH game with the extended reduction 
+adversary.\<close>
+lemma bind_game_eq_t_BSDH_red: "bind_game \<A> = t_BSDH.game (ext_reduction \<A>)"
 proof - 
   note [simp] = Let_def split_def
 
@@ -255,9 +296,11 @@ proof -
   and the public key\<close>
   let ?mr = "\<lambda>\<alpha>. (of_int_mod_ring (int \<alpha>)::'e mod_ring)"
   let ?PK = "\<lambda>\<alpha>. (map (\<lambda>t. \<^bold>g\<^bsub>G\<^sub>p\<^esub> ^\<^bsub>G\<^sub>p\<^esub> ((?mr \<alpha>)^t)) [0..<max_deg+1])"
-  have "t_BSDH.game (bind_reduction \<A>) =  TRY do { 
+
+  text \<open>Firstly, unfold the t-BSDH game and the reduction adversary\<close>
+  have "t_BSDH.game (ext_reduction \<A>) =  TRY do { 
     \<alpha> \<leftarrow> sample_uniform (order G\<^sub>p);
-    (c, g) \<leftarrow> (bind_reduction \<A>) (?PK \<alpha>);
+    (c, g) \<leftarrow> (ext_reduction \<A>) (?PK \<alpha>);
     _::unit \<leftarrow> assert_spmf((e \<^bold>g \<^bold>g) ^\<^bsub>G\<^sub>T\<^esub> (1/((?mr \<alpha>)+c)) = g);
     return_spmf True 
   } ELSE return_spmf False"
@@ -319,6 +362,7 @@ proof -
   } ELSE return_spmf False"
    unfolding split_def Let_def
    by(fold try_bind_spmf_lossless2[OF lossless_return_spmf]) simp
+ text \<open>erase the pairing check with he literal helping lemma to get closer to the eval bind game\<close>
   also have "\<dots> = TRY do { 
     \<alpha> \<leftarrow> sample_uniform (order G\<^sub>p);
     (C, i, \<phi>_i, w_i, B, w_B, r_x) \<leftarrow> \<A> (?PK \<alpha>);
@@ -327,6 +371,7 @@ proof -
     return_spmf True  
   } ELSE return_spmf False"
     unfolding Let_def using literal_helping by algebra 
+  text \<open>Split the message checks off the Evaluations checks, as it is done in the eval bind game\<close>
   also have "\<dots> = TRY do { 
     \<alpha> \<leftarrow> sample_uniform (order G\<^sub>p);
     TRY do {
@@ -361,14 +406,75 @@ proof -
   } ELSE return_spmf False" 
   unfolding split_def Let_def
   by(fold try_bind_spmf_lossless2[OF lossless_return_spmf]) simp
+  text \<open>the obtained game is already the evaluation binding game.\<close>
   also have "\<dots>= bind_game \<A>"
     using bind_game_alt_def unfolding KeyGen_def Setup_def by simp
   finally show ?thesis ..
 qed
 
-theorem batchOpening_binding: "bind_advantage \<A> = t_BSDH.advantage (bind_reduction \<A>)"
+text \<open>From the previous lemma we conclude that the adversarys advantage on winning the evaluation 
+binding game is the same as winning the t-BSDH game with the extended reduction adversary.\<close>
+lemma evaluation_binding_ext_red: "bind_advantage \<A> = t_BSDH.advantage (ext_reduction \<A>)"
   unfolding bind_advantage_def t_BSDH.advantage_def
   using bind_game_eq_t_BSDH_red by presburger
+
+text \<open>Now we use overestimation to show that the advantage of winning the t-BSDH game with the 
+extended reduction adversary is less than or equal to winning it with the normal reduction adversary.\<close>
+lemma overestimate_reductions: "spmf (t_BSDH.game (ext_reduction \<A>)) True 
+  \<le> spmf (t_BSDH.game (reduction \<A>)) True"
+  (is "spmf ?lhgame True \<le> spmf ?rhgame True")
+proof -
+  note [simp] = Let_def split_def
+
+  text \<open>abbreviations for the mod_ring version of sample uniform nat 
+  and the public key\<close>
+  let ?\<alpha> = "\<lambda>\<alpha>. (of_int_mod_ring (int \<alpha>)::'e mod_ring)"
+  let ?PK = "\<lambda>\<alpha>. (map (\<lambda>t. \<^bold>g\<^bsub>G\<^sub>p\<^esub> ^\<^bsub>G\<^sub>p\<^esub> ((?\<alpha> \<alpha>)^t)) [0..<max_deg+1])"
+
+  text \<open>We extend the t-BSDH game with the extended reduction adversary to a complete game.\<close>
+  have bind_red_ext: "t_BSDH.game (ext_reduction \<A>) = TRY do { 
+    \<alpha> \<leftarrow> sample_uniform (order G\<^sub>p);
+    (C, i, \<phi>_i, w_i, B, w_B, r_x) \<leftarrow> \<A> (?PK \<alpha>);
+    _ :: unit \<leftarrow> assert_spmf (i \<in> B \<and> \<phi>_i \<noteq> poly r_x i \<and> valid_msg \<phi>_i w_i \<and> valid_batch_msg r_x w_B B
+                              \<and> VerifyEval (?PK \<alpha>) C i \<phi>_i w_i \<and> VerifyEvalBatch (?PK \<alpha>) C B r_x w_B);
+    let p' = g_pow_PK_Prod (?PK \<alpha>) (prod (\<lambda>i. [:-i,1:]) B div [:-i,1:]);
+    let r' = g_pow_PK_Prod (?PK \<alpha>) ((r_x - [:poly r_x i:]) div [:-i,1:]);
+    _::unit \<leftarrow>  assert_spmf ((e \<^bold>g \<^bold>g) ^\<^bsub>G\<^sub>T\<^esub> (1/((?\<alpha> \<alpha>)+(-i))) = (e p' w_B \<otimes>\<^bsub>G\<^sub>T\<^esub> e (r' \<div>\<^bsub>G\<^sub>p\<^esub> w_i) \<^bold>g) ^\<^bsub>G\<^sub>T\<^esub> (1/(\<phi>_i - poly r_x i))); 
+    return_spmf True  
+  } ELSE return_spmf False"
+    by (force simp add: t_BSDH.game_alt_def[of "(ext_reduction \<A>)"])
+
+  text \<open>We extend the t-BSDH game with reduction adversary to a complete game.\<close>
+  have eval_bind_red_ext: "t_BSDH.game (reduction \<A>) = TRY do { 
+    \<alpha> \<leftarrow> sample_uniform (order G\<^sub>p);
+    (C, i, \<phi>_i, w_i, B, w_B, r_x) \<leftarrow> \<A> (?PK \<alpha>);
+    let p' = g_pow_PK_Prod (?PK \<alpha>) (prod (\<lambda>i. [:-i,1:]) B div [:-i,1:]);
+    let r' = g_pow_PK_Prod (?PK \<alpha>) ((r_x - [:poly r_x i:]) div [:-i,1:]);
+    _::unit \<leftarrow>  assert_spmf ((e \<^bold>g \<^bold>g) ^\<^bsub>G\<^sub>T\<^esub> (1/((?\<alpha> \<alpha>)+(-i))) = (e p' w_B \<otimes>\<^bsub>G\<^sub>T\<^esub> e (r' \<div>\<^bsub>G\<^sub>p\<^esub> w_i) \<^bold>g) ^\<^bsub>G\<^sub>T\<^esub> (1/(\<phi>_i - poly r_x i))); 
+    return_spmf True  
+  } ELSE return_spmf False"
+    by (force simp add: t_BSDH.game_alt_def[of "(reduction \<A>)"])
+
+  text \<open>We show the thesis in ennreal, which implies the plain thesis\<close>
+  have "ennreal (spmf (t_BSDH.game (ext_reduction \<A>)) True) 
+    \<le> ennreal (spmf (t_BSDH.game (reduction \<A>)) True)"
+    unfolding bind_red_ext eval_bind_red_ext
+    apply (simp add: spmf_try_spmf ennreal_spmf_bind)
+    apply (rule nn_integral_mono)+
+    apply (simp add: assert_spmf_def)
+    apply (simp add: measure_spmf.emeasure_eq_measure)
+    done
+
+  then show ?thesis by simp
+qed
+
+text \<open>Finally we put everything together: 
+we conclude that for every efficient adversary the advantage of winning the 
+evaluation binding game for the batched KZG is less than or equal to breaking the t-BSDH assumption.\<close>
+theorem evaluation_binding: "bind_advantage \<A> \<le> t_BSDH.advantage (reduction \<A>)"
+  using evaluation_binding_ext_red overestimate_reductions
+  unfolding t_BSDH.advantage_def
+  by algebra
 
 end 
 
